save

DP_Pred.thy
@@ -7,8 +7,50 @@ context
   includes lifting_syntax
 begin
   
+definition consistentPred :: "('a \<Rightarrow> bool) \<Rightarrow> ('param \<rightharpoonup> 'result, 'a) state \<Rightarrow> bool" where
+  "consistentPred P s \<equiv> \<forall>M. consistentM M \<longrightarrow> (case runState s M of (v', M') \<Rightarrow> P v' \<and> consistentM M')"
   
+definition consistentPred_alt :: "('a \<Rightarrow> bool) \<Rightarrow> ('param \<rightharpoonup> 'result, 'a) state \<Rightarrow> bool" where
+  "consistentPred_alt P s \<equiv> pred_fun consistentM (pred_prod P consistentM) (runState s)"
   
+lemma "consistentPred_alt = consistentPred"
+  unfolding consistentPred_def consistentPred_alt_def
+  by (fastforce split: pred_prod_split)
+term 0(**)
+
+notation pred_fun (infixr "...>" 55)
+
+abbreviation pred_fun_lifted :: "('a \<Rightarrow> bool) \<Rightarrow> ('b \<Rightarrow> bool) \<Rightarrow> ('a ==_\<Longrightarrow> 'b) \<Rightarrow> bool" (infixr "...>\<^sub>T" 55) where
+  "A ...>\<^sub>T B \<equiv> A ...> consistentPred B"
+
+  
+lemma consistentPred_intro:
+  assumes "\<And>M v' M'. \<lbrakk>consistentM M; runState v\<^sub>T M = (v', M')\<rbrakk> \<Longrightarrow> P v' \<and> consistentM M'"
+  shows "consistentPred P v\<^sub>T"
+  unfolding consistentPred_def using assms by blast
+
+lemma consistentPred_elim:
+  assumes "consistentPred P v\<^sub>T" "consistentM M"
+  obtains v' M' where "runState v\<^sub>T M = (v', M')" "P v'" "consistentM M'"
+  using assms unfolding consistentPred_def by blast
+term 0 (**)
+
+lemma consistentPred_return:
+  "P v \<Longrightarrow> consistentPred P \<langle>v\<rangle>"
+  unfolding return_def by (fastforce intro: consistentPred_intro)
+
+lemma return_transferP:
+  "(P ...> consistentPred P) return"
+  unfolding pred_fun_def by (metis consistentPred_return)
+    
+lemma bind_transferP:
+  "(consistentPred P0 ...> (P0 ...>\<^sub>T P1) ...> consistentPred P1) (op \<bind>)"
+  unfolding bind_def pred_fun_def by (fastforce intro: consistentPred_intro elim: consistentPred_elim split: prod.split)
+    
+lemma fun_app_lifted_transferP:
+  "(consistentPred (R0 ...>\<^sub>T R1) ...> consistentPred P0 ...> consistentPred P1) (op .)"
+  unfolding fun_app_lifted_def
+  oops 
 end
 end
 end
